theories/typing/examples/lazy_lft.v
@@ -19,7 +19,7 @@ Section lazy_lft.
 
   Lemma lazy_lft_type : typed_val lazy_lft (fn(∅) → unit).
   Proof.
-    intros. iApply type_fn; [solve_typing..|]. iIntros "/= !#".
+    intros E L. iApply type_fn; [solve_typing..|]. iIntros "/= !#".
       iIntros ([] ϝ ret p). inv_vec p. simpl_subst.
     iApply (type_newlft []). iIntros (α).
     iApply (type_new_subtype (Π[uninit 1;uninit 1])); [solve_typing..|].
