theories/typing/lib/option.v
@@ -26,7 +26,7 @@ Section option.
     typed_val
       option_as_mut (fn(∀ α, ∅; &uniq{α} (option τ)) → option (&uniq{α}τ)).
   Proof.
-    intros. iApply type_fn; [solve_typing..|]. iIntros "/= !#". iIntros (α ϝ ret p).
+    intros E L. iApply type_fn; [solve_typing..|]. iIntros "/= !#". iIntros (α ϝ ret p).
       inv_vec p=>o. simpl_subst.
     iApply type_deref; [solve_typing..|]. iIntros (o'). simpl_subst.
     iApply type_new; [solve_typing..|]. iIntros (r). simpl_subst.
@@ -56,7 +56,7 @@ Section option.
   Lemma option_unwrap_or_type τ `{!TyWf τ} :
     typed_val (option_unwrap_or τ) (fn(∅; option τ, τ) → τ).
   Proof.
-    intros. iApply type_fn; [solve_typing..|]. iIntros "/= !#".
+    intros E L. iApply type_fn; [solve_typing..|]. iIntros "/= !#".
       iIntros ([] ϝ ret p). inv_vec p=>o def. simpl_subst.
     iApply type_case_own; [solve_typing|]. constructor; last constructor; last constructor.
     + right. iApply type_delete; [solve_typing..|].
