theories/typing/lib/rwlock/rwlock_code.v
@@ -22,7 +22,7 @@ Section rwlock_functions.
   Lemma rwlock_new_type ty `{!TyWf ty} :
     typed_val (rwlock_new ty) (fn(∅; ty) → rwlock ty).
   Proof.
-    intros. iApply type_fn; [solve_typing..|]. iIntros "/= !#".
+    intros E L. iApply type_fn; [solve_typing..|]. iIntros "/= !#".
       iIntros (_ ret ϝ arg). inv_vec arg=>x. simpl_subst.
     iApply type_new; [solve_typing..|].
     iIntros (r tid) "#LFT HE Hna HL Hk HT". simpl_subst.
@@ -58,7 +58,7 @@ Section rwlock_functions.
   Lemma rwlock_into_inner_type ty `{!TyWf ty} :
     typed_val (rwlock_into_inner ty) (fn(∅; rwlock ty) → ty).
   Proof.
-    intros. iApply type_fn; [solve_typing..|]. iIntros "/= !#".
+    intros E L. iApply type_fn; [solve_typing..|]. iIntros "/= !#".
       iIntros (_ ret ϝ arg). inv_vec arg=>x. simpl_subst.
     iApply type_new; [solve_typing..|].
     iIntros (r tid) "#LFT HE Hna HL Hk HT". simpl_subst.
@@ -92,7 +92,7 @@ Section rwlock_functions.
   Lemma rwlock_get_mut_type ty `{!TyWf ty} :
     typed_val rwlock_get_mut (fn(∀ α, ∅; &uniq{α} (rwlock ty)) → &uniq{α} ty).
   Proof.
-    intros. iApply type_fn; [solve_typing..|]. iIntros "/= !#".
+    intros E L. iApply type_fn; [solve_typing..|]. iIntros "/= !#".
       iIntros (α ϝ ret arg). inv_vec arg=>x. simpl_subst.
     iApply type_deref; [solve_typing..|]. iIntros (x'). simpl_subst.
     iIntros (tid) "#LFT HE Hna HL HC HT".
@@ -143,7 +143,7 @@ Section rwlock_functions.
     typed_val rwlock_try_read
         (fn(∀ α, ∅; &shr{α}(rwlock ty)) → option (rwlockreadguard α ty)).
   Proof.
-    intros. iApply type_fn; [solve_typing..|]. iIntros "/= !#".
+    intros E L. iApply type_fn; [solve_typing..|]. iIntros "/= !#".
       iIntros (α ϝ ret arg). inv_vec arg=>x. simpl_subst.
     iApply type_new; [solve_typing..|]. iIntros (r). simpl_subst.
     iApply type_deref; [solve_typing..|]. iIntros (x'). simpl_subst.
@@ -258,7 +258,7 @@ Section rwlock_functions.
     typed_val rwlock_try_write
         (fn(∀ α, ∅; &shr{α}(rwlock ty)) → option (rwlockwriteguard α ty)).
   Proof.
-    intros. iApply type_fn; [solve_typing..|]. iIntros "/= !#".
+    intros E L. iApply type_fn; [solve_typing..|]. iIntros "/= !#".
       iIntros (α ϝ ret arg). inv_vec arg=>x. simpl_subst.
     iApply (type_cont [_] [ϝ ⊑ₗ []] (λ r, [x ◁ box (&shr{α} rwlock ty);
                                         r!!!0 ◁ box (option (rwlockwriteguard α ty))]));
