theories/typing/lib/rwlock/rwlockreadguard_code.v
@@ -20,9 +20,9 @@ Section rwlockreadguard_functions.
 
   Lemma rwlockreadguard_deref_type ty `{!TyWf ty} :
     typed_val rwlockreadguard_deref
-      (fn (fun '(α, β) => FP_wf ∅ [# &shr{α}(rwlockreadguard β ty)] (&shr{α}ty))).
+      (fn(∀ '(α, β), ∅; &shr{α} rwlockreadguard β ty) → &shr{α} ty).
   Proof.
-    intros. iApply type_fn; [solve_typing..|]. iIntros "/= !#".
+    intros E L. iApply type_fn; [solve_typing..|]. iIntros "/= !#".
       iIntros ([α β] ϝ ret arg). inv_vec arg=>x. simpl_subst.
     iApply type_deref; [solve_typing..|]. iIntros (x').
     iIntros (tid) "#LFT #HE Hna HL Hk HT". simpl_subst.
@@ -61,7 +61,7 @@ Section rwlockreadguard_functions.
   Lemma rwlockreadguard_drop_type ty `{!TyWf ty} :
     typed_val rwlockreadguard_drop (fn(∀ α, ∅; rwlockreadguard α ty) → unit).
   Proof.
-    intros. iApply type_fn; [solve_typing..|]. iIntros "/= !#".
+    intros E L. iApply type_fn; [solve_typing..|]. iIntros "/= !#".
       iIntros (α ϝ ret arg). inv_vec arg=>x. simpl_subst.
     iApply type_deref; [solve_typing..|]. iIntros (x'). simpl_subst.
     iApply (type_cont [] [ϝ ⊑ₗ []] (λ _, [x ◁ _; x' ◁ _]));
