theories/typing/lib/rwlock/rwlockwriteguard_code.v
@@ -20,9 +20,9 @@ Section rwlockwriteguard_functions.
 
   Lemma rwlockwriteguard_deref_type ty `{!TyWf ty} :
     typed_val rwlockwriteguard_deref
-      (fn (fun '(α, β) => FP_wf ∅ [# &shr{α}(rwlockwriteguard β ty)] (&shr{α}ty))).
+      (fn(∀ '(α, β), ∅; &shr{α} rwlockwriteguard β ty) → &shr{α} ty).
   Proof.
-    intros. iApply type_fn; [solve_typing..|]. iIntros "/= !#".
+    intros E L. iApply type_fn; [solve_typing..|]. iIntros "/= !#".
       iIntros ([α β] ϝ ret arg). inv_vec arg=>x. simpl_subst.
     iApply type_deref; [solve_typing..|]. iIntros (x').
     iIntros (tid) "#LFT #HE Hna HL Hk HT". simpl_subst.
@@ -64,9 +64,9 @@ Section rwlockwriteguard_functions.
 
   Lemma rwlockwriteguard_derefmut_type ty `{!TyWf ty} :
     typed_val rwlockwriteguard_derefmut
-      (fn (fun '(α, β) => FP_wf ∅ [# &uniq{α}(rwlockwriteguard β ty)] (&uniq{α}ty))).
+      (fn(∀ '(α, β), ∅; &uniq{α} rwlockwriteguard β ty) → &uniq{α} ty).
   Proof.
-    intros. iApply type_fn; [solve_typing..|]. iIntros "/= !#".
+    intros E L. iApply type_fn; [solve_typing..|]. iIntros "/= !#".
       iIntros ([α β] ϝ ret arg). inv_vec arg=>x. simpl_subst.
     iApply type_deref; [solve_typing..|]. iIntros (x').
     iIntros (tid) "#LFT #HE Hna HL Hk HT". simpl_subst.
@@ -111,7 +111,7 @@ Section rwlockwriteguard_functions.
     typed_val rwlockwriteguard_drop
               (fn(∀ α, ∅; rwlockwriteguard α ty) → unit).
   Proof.
-    intros. iApply type_fn; [solve_typing..|]. iIntros "/= !#".
+    intros E L. iApply type_fn; [solve_typing..|]. iIntros "/= !#".
       iIntros (α ϝ ret arg). inv_vec arg=>x. simpl_subst.
     iApply type_deref; [solve_typing..|]. iIntros (x'). simpl_subst.
     iIntros (tid) "#LFT #HE Hna HL Hk HT".
